Update closureCLC.lean

CLLean/Completeness/closureCLC.lean
@@ -11,26 +11,26 @@ if ψ ∈ cl φ and subformula χ ψ, then we must have χ ∈ cl φ .
 import CLLean.Syntax.syntaxCLC
 import CLLean.Syntax.propLemmas
 
-open Classical Set axCLC
+open Classical Set axCLC formCLC
 
 ----------------------------------------------------------
 -- Filtration closure cl
 ----------------------------------------------------------
-noncomputable def cl_C {agents : Type} [hN : Fintype agents] (G : Set (agents))
+noncomputable def cl_C {agents : Type} [Fintype agents] (G : Set (agents))
   (φ : formCLC agents) : Finset (formCLC agents) :=
 Finset.image (λ i => _K (i) (_C G φ)) (toFinset G) ∪
   Finset.image (λ i => (_¬ _K (i) (_C G φ))) (toFinset G)
 
-noncomputable def cl {agents : Type} [hN : Fintype agents] :
+noncomputable def cl {agents : Type} [Fintype agents] :
   formCLC agents → Finset (formCLC agents)
 |  _⊥              => {_⊥, _¬ _⊥}
-| (formCLC.var n)  => {formCLC.var n, _¬ (formCLC.var n), _⊥, _¬ _⊥}
+| (var n)          => {var n, _¬ (var n), _⊥, _¬ _⊥}
 | (φ _→ ψ)         => cl φ ∪ cl ψ ∪ (ite (ψ = _⊥) {(φ _→ _⊥)} {(φ _→ ψ), _¬ (φ _→ ψ)})
 | (φ _∧ ψ)         => cl φ ∪ cl ψ ∪ {(φ _∧ ψ), _¬ (φ _∧ ψ)}
 | (_[G] φ)         => cl φ ∪ {(_[G] φ), _¬ _[G] φ} ∪
                         {(_C (G) (_[G] φ)), _¬ (_C (G) (_[G] φ))} ∪ cl_C G (_[G] φ)
-| (formCLC.K i φ) => cl φ ∪ {(_K i φ), _¬ (_K i φ)}
-| (_C G φ)        => cl φ ∪ {(_C G φ), _¬ (_C G φ)} ∪ cl_C G φ
+| (formCLC.K i φ)  => cl φ ∪ {(_K i φ), _¬ (_K i φ)}
+| (_C G φ)         => cl φ ∪ {(_C G φ), _¬ (_C G φ)} ∪ cl_C G φ
 
 ----------------------------------------------------------
 -- Lemmas about cl
@@ -42,11 +42,11 @@ noncomputable def cl {agents : Type} [hN : Fintype agents] :
     simp_all only [cl, Finset.union_insert, Finset.mem_union, Finset.mem_insert, Finset.mem_singleton, or_false,
     eq_self_iff_true, and_self, or_true, true_or, Finset.mem_union, Finset.union_assoc]
   · unfold cl
-    simp only [Finset.mem_singleton, formCLC.imp.injEq, Finset.union_assoc, Finset.mem_union]
+    simp only [Finset.mem_singleton, imp.injEq, Finset.union_assoc, Finset.mem_union]
     split_ifs with h
-    simp only [Finset.mem_singleton, formCLC.imp.injEq, h, and_false, Finset.mem_insert,
+    simp only [Finset.mem_singleton, imp.injEq, h, and_false, Finset.mem_insert,
       or_false, or_true]
-    simp only [Finset.mem_singleton, formCLC.imp.injEq, Finset.mem_insert, true_or, or_true]
+    simp only [Finset.mem_singleton, imp.injEq, Finset.mem_insert, true_or, or_true]
 
 
 
@@ -76,7 +76,7 @@ lemma cl_C_contains_KC {agents : Type} [hN : Fintype agents] {φ ψ : formCLC ag
     · simp only [Finset.mem_insert, Finset.mem_singleton, or_self] at h
   · simp only [Finset.mem_singleton, Finset.union_insert, Finset.mem_union, or_false,
     Finset.insert_union, Finset.union_assoc, or_self, Finset.mem_insert, false_or,
-    formCLC.C.injEq] at *
+    C.injEq] at *
     cases' h with h h
     · rw [h.1] at hi
       simp [h.1, h.2, cl_C, hi, Finset.mem_union, Finset.mem_image, mem_toFinset, eq_self_iff_true,
@@ -86,11 +86,11 @@ lemma cl_C_contains_KC {agents : Type} [hN : Fintype agents] {φ ψ : formCLC ag
     simp only [cl_C, Finset.mem_union, Finset.mem_image, mem_toFinset, and_false, exists_false,
       or_self] at h
   · simp only [Finset.mem_singleton, Finset.union_insert, Finset.mem_union, or_false,
-      Finset.mem_insert, false_or, formCLC.K.injEq] at *
+      Finset.mem_insert, false_or, K.injEq] at *
     exact Or.inr (ih h)
   · simp only [Finset.mem_singleton, Finset.union_insert, Finset.mem_union, or_false, cl_C,
       Finset.insert_union, Finset.union_assoc, Finset.mem_image, mem_toFinset, and_false,
-      exists_false, or_self, Finset.mem_insert, formCLC.C.injEq, formCLC.K.injEq, false_or] at *
+      exists_false, or_self, Finset.mem_insert, C.injEq, K.injEq, false_or] at *
     cases' h with h h
     · rw [h.1] at hi
       simp only [h.1, h.2, and_true, exists_eq_right, hi, or_true]
@@ -99,178 +99,186 @@ lemma cl_C_contains_KC {agents : Type} [hN : Fintype agents] {φ ψ : formCLC ag
 lemma cl_closed_single_neg {agents : Type} [hN : Fintype agents]
   (φ x : formCLC agents) (hx : x ∈ cl φ) :
   ∃ ψ, (ψ ∈ cl φ ∧ _⊢ (ψ _↔ (_¬ x))) := by
-  induction' φ with _ _ _ ih_φ ih_ψ _ _ ih_φ ih_ψ _ _ ih _ _ ih _ _ ih
-  repeat'
-    · unfold cl at *
-      simp only [Finset.union_insert, Finset.insert_union, Finset.union_assoc, Finset.mem_insert,
-                  Finset.mem_union, Finset.mem_singleton] at hx
-      cases' hx with hx hx
-      · apply Exists.intro (_¬ x)
-        simp only [hx, Finset.mem_insert, Finset.mem_union, Finset.mem_singleton, eq_self_iff_true
-                    false_or, true_or, or_true, true_and] at *
-        exact iff_iden --apply @iff_iden (formCLC agents) _ _
+  induction' φ with n φ ψ ih_φ ih_ψ φ ψ ih_φ ih_ψ G φ ih i φ ih G φ ih
+  all_goals try
+    unfold cl at hx ⊢
+    simp only [Finset.union_insert, Finset.insert_union, Finset.union_assoc, Finset.mem_insert,
+                Finset.mem_union, Finset.mem_singleton] at hx
+    cases' hx with hx hx
+    apply Exists.intro (_¬ x)
+    simp only [hx, Finset.mem_insert, Finset.mem_union, Finset.mem_singleton, eq_self_iff_true
+                false_or, true_or, or_true, true_and] at *
+    apply @iff_iden (formCLC agents) _ _
+
   · apply Exists.intro (_⊥)
-    -- simp only [hx, Finset.mem_insert, eq_self_iff_true, Finset.mem_singleton, or_false, true_and]
+    simp only [hx, Finset.mem_insert, eq_self_iff_true, Finset.mem_singleton, or_false, true_and]
     apply MP
     apply MP
     apply Prop4
     exact @dni (formCLC agents) _ _
     exact @nnn_bot (formCLC agents) _
-  · cases hx
-   · apply Exists.intro (var φ)
-      simp only [hx, Finset.mem_insert, eq_self_iff_true, Finset.mem_singleton
+  · cases' hx with hx hx
+    · apply Exists.intro (var n)
+      simp only [hx, Finset.mem_insert, eq_self_iff_true, Finset.mem_singleton,
                   or_false, true_and] at *
       exact @iff_dni (formCLC agents) _ _
-    cases hx
-    · apply Exists.intro ('⊤)
-      simp only [hx, Finset.mem_insert, eq_self_iff_true, false_and, Finset.mem_singleton
-                  false_or, true_and]
+    cases' hx with hx hx
+    · apply Exists.intro (_⊤)
+      simp only [Finset.mem_singleton, Finset.mem_insert, imp.injEq, and_true, or_self, or_true, hx,
+        true_and]
       apply @iff_iden (formCLC agents) _ _
     · apply Exists.intro (_⊥)
-      simp only [hx, Finset.mem_insert, eq_self_iff_true, Finset.mem_singleton, or_false
+      simp only [hx, Finset.mem_insert, eq_self_iff_true, Finset.mem_singleton, or_false,
                   false_or, true_and]
       apply MP
-    apply MP
-    apply Prop4
-    exact @dni (formCLC agents) _ _
-    exact @nnn_bot (formCLC agents) _
-  · cases hx
-    · specialize φ_ih_φ hx
-      cases φ_ih_φ with ψ hψ
+      apply MP
+      apply Prop4
+      exact @dni (formCLC agents) _ _
+      exact @nnn_bot (formCLC agents) _
+  · cases' hx with hx hx
+    · specialize ih_φ hx
+      cases' ih_φ with ψ hψ
       apply Exists.intro ψ
-      split
+      apply And.intro
       apply Finset.mem_union_left
       apply Finset.mem_union_left
       exact hψ.1
       exact hψ.2
-    cases hx
-    · specialize φ_ih_ψ hx
-      cases φ_ih_ψ with ψ hψ
+    cases' hx with hx hx
+    · specialize ih_ψ hx
+      cases' ih_ψ with ψ hψ
       apply Exists.intro ψ
-      split
+      apply And.intro
       apply Finset.mem_union_left
       apply Finset.mem_union_right
       exact hψ.1
       exact hψ.2
-      · apply Exists.intro (φ_φ _∧ φ_ψ)
-        simp only [hx, Finset.union_insert, Finset.mem_insert, eq_self_iff_true
-                    true_or, true_and]
-        exact @iff_dni (formCLC agents) _ _
-  · unfold cl at *
+    · apply Exists.intro (φ _∧ ψ)
+      simp only [Finset.mem_singleton, Finset.union_insert, Finset.union_assoc, Finset.mem_union,
+        or_false, Finset.mem_insert, true_or, hx, true_and]
+      exact @iff_dni (formCLC agents) _ _
+  · unfold cl at hx ⊢
     simp only [Finset.union_assoc, Finset.mem_union] at hx
-    cases hx
-    · specialize φ_ih_φ hx
-      cases φ_ih_φ with ψ hψ
+    cases' hx with hx hx
+    · specialize ih_φ hx
+      cases' ih_φ with ψ hψ
       apply Exists.intro ψ
-      split
+      apply And.intro
       apply Finset.mem_union_left
       apply Finset.mem_union_left
       exact hψ.1
       exact hψ.2
-    cases hx
-    · specialize φ_ih_ψ hx
-      cases φ_ih_ψ with ψ hψ
+    cases' hx with hx hx
+    · specialize ih_ψ hx
+      cases' ih_ψ with ψ hψ
       apply Exists.intro ψ
-      split
+      apply And.intro
       apply Finset.mem_union_left
       apply Finset.mem_union_right
       exact hψ.1
       exact hψ.2
-    · split_ifs at hx
-      · simp only [h, eq_self_iff_true, if_true, Finset.union_assoc, Finset.mem_union
+    · split_ifs at hx with h
+      · simp only [h, eq_self_iff_true, if_true, Finset.union_assoc, Finset.mem_union,
                     Finset.mem_singleton] at *
         simp only [hx]
-        apply Exists.intro (φ_φ)
-        split
-        apply or.intro_left
-        exact cl_contains_phi φ_φ
+        apply Exists.intro (φ)
+        apply And.intro
+        apply Or.intro_left
+        exact cl_contains_phi φ
         exact @iff_dni (formCLC agents) _ _
-      · simp only [h, if_false, Finset.union_insert, Finset.union_assoc, Finset.mem_insert
+      · simp only [h, if_false, Finset.union_insert, Finset.union_assoc, Finset.mem_insert,
                     Finset.mem_union, Finset.mem_singleton, not_false_iff] at *
-        cases hx
-        · apply Exists.intro (_¬ (φ_φ _→ φ_ψ))
+        cases' hx with hx hx
+        · apply Exists.intro (_¬ (φ _→ ψ))
           simp only [hx, eq_self_iff_true, or_true, true_and]
           exact @iff_iden (formCLC agents) _ _
-        · apply Exists.intro (φ_φ _→ φ_ψ)
+        · apply Exists.intro (φ _→ ψ)
           simp only [hx, eq_self_iff_true, true_or, true_and]
           exact @iff_dni (formCLC agents) _ _
-  · cases hx
-    · apply Exists.intro (_¬ (_C φ_G '[φ_G] φ_φ))
-      simp only [hx, Finset.mem_insert, Finset.mem_union, Finset.mem_singleton, eq_self_iff_true
-                  true_or, or_true, true_and]
+  · cases' hx with hx hx
+    · apply Exists.intro (_¬ (_[G] φ))
+      simp only [Finset.mem_singleton, Finset.union_insert, Finset.mem_union, or_false,
+        Finset.insert_union, Finset.union_assoc, or_self, Finset.mem_insert, false_or, imp.injEq,
+        and_true, true_or, or_true, hx, true_and]
       exact @iff_iden (formCLC agents) _ _
-    cases hx
-    · specialize φ_ih hx
-      cases φ_ih with ψ hψ
+    cases' hx with hx hx
+    · specialize ih hx
+      cases' ih with ψ hψ
       apply Exists.intro ψ
-      split
+      apply And.intro
       apply Finset.mem_union_left
       apply Finset.mem_union_left
       apply Finset.mem_union_left
       exact hψ.1
       exact hψ.2
-    cases hx
-    · apply Exists.intro ('[φ_G] φ_φ)
-      simp only [hx, Finset.union_insert, Finset.mem_insert, eq_self_iff_true, Finset.mem_union
+    cases' hx with hx hx
+    · apply Exists.intro (_[G] φ)
+      simp only [hx, Finset.union_insert, Finset.mem_insert, eq_self_iff_true, Finset.mem_union,
                   false_or, true_or, true_and]
       exact @iff_dni (formCLC agents) _ _
-    cases hx
-    · apply Exists.intro (_C φ_G '[φ_G] φ_φ)
-        simp only [hx, Finset.union_insert, Finset.mem_insert, eq_self_iff_true, Finset.mem_union
-                    false_or, true_or, true_and]
-        exact @iff_dni (formCLC agents) _ _
-    · unfold cl_C at *
-      simp only [Finset.mem_union, Finset.mem_image, mem_to_finset, exists_prop] at hx
-      cases hx
-      · cases hx with i hi
-        apply Exists.intro (_¬ _K i (_C φ_G ('[φ_G]φ_φ)))
-        simp only [hi.left, ←hi.right, Finset.mem_union, eq_self_iff_true, Finset.mem_image
-                    mem_to_finset, and_true, exists_prop, exists_eq_right, or_true, true_and]
+    cases' hx with hx hx
+    · apply Exists.intro (_C G (_[G] φ))
+      simp only [hx, Finset.union_insert, Finset.mem_insert, eq_self_iff_true, Finset.mem_union,
+                  false_or, true_or, true_and]
+      exact @iff_dni (formCLC agents) _ _
+    · unfold cl_C at hx ⊢
+      simp only [Finset.mem_union, Finset.mem_image, mem_toFinset, exists_prop] at hx
+      cases' hx with hx hx
+      · cases' hx with i hi
+        apply Exists.intro (_¬ _K i (_C G (_[G]φ)))
+        simp only [Finset.mem_singleton, Finset.union_insert, Finset.mem_union, or_false,
+          Finset.insert_union, Finset.union_assoc, or_self, Finset.mem_insert, false_or,
+          Finset.mem_image, mem_toFinset, and_false, exists_false, imp.injEq, and_true, K.injEq,
+          exists_eq_right, hi.1, or_true, ← hi.2, true_and]
         exact @iff_iden (formCLC agents) _ _
-      · cases hx with i hi
-        apply Exists.intro (_K i (_C φ_G ('[φ_G]φ_φ)))
-        simp only [hi.left, ←hi.right, Finset.mem_union, Finset.mem_image, mem_to_finset
-                    eq_self_iff_true, and_true, exists_prop, exists_eq_right, exists_false
-                    or_false, or_true, true_and]
+      · cases' hx with i hi
+        apply Exists.intro (_K i (_C G (_[G]φ)))
+        simp only [Finset.mem_singleton, Finset.union_insert, Finset.mem_union, or_false,
+          Finset.insert_union, Finset.union_assoc, or_self, Finset.mem_insert, false_or,
+          Finset.mem_image, mem_toFinset, and_false, exists_false, K.injEq, and_true,
+          exists_eq_right, hi.1, or_true, ← hi.2, true_and]
         exact @iff_dni (formCLC agents) _ _
-  · cases hx
-    · specialize φ_ih hx
-      cases φ_ih with ψ hψ
+  · cases' hx with hx hx
+    · specialize ih hx
+      cases' ih with ψ hψ
       apply Exists.intro ψ
-      split
+      apply And.intro
       apply Finset.mem_union_left
       exact hψ.1
       exact hψ.2
-    · apply Exists.intro (_K φ_a φ_φ)
+    · apply Exists.intro (_K i φ)
       simp only [hx, Finset.union_insert, Finset.mem_insert, eq_self_iff_true, true_or, true_and]
       exact @iff_dni (formCLC agents) _ _
-  · cases hx
-    · specialize φ_ih hx
-      cases φ_ih with ψ hψ
+  · cases' hx with hx hx
+    · specialize ih hx
+      cases' ih with ψ hψ
       apply Exists.intro ψ
-      split
+      apply And.intro
       apply Finset.mem_union_left
       apply Finset.mem_union_left
       exact hψ.1
       exact hψ.2
-    cases hx
-    · apply Exists.intro ((_C φ_G (φ_φ)))
-      simp only [hx, Finset.union_insert, Finset.mem_insert, eq_self_iff_true, Finset.mem_union
+    cases' hx with hx hx
+    · apply Exists.intro ((_C G (φ)))
+      simp only [hx, Finset.union_insert, Finset.mem_insert, eq_self_iff_true, Finset.mem_union,
                   true_or, true_and]
       exact @iff_dni (formCLC agents) _ _
     · unfold cl_C at *
-      simp only [Finset.mem_union, Finset.mem_image, mem_to_finset, exists_prop] at hx
-      cases hx
-      · cases hx with i hi
-        apply Exists.intro (_¬ _K i (_C φ_G φ_φ))
-        simp only [hi.left, ←hi.right, Finset.mem_union, eq_self_iff_true, Finset.mem_image
-                    mem_to_finset, and_true, exists_prop, exists_eq_right, or_true, true_and]
+      simp only [Finset.mem_union, Finset.mem_image, mem_toFinset, exists_prop] at hx
+      cases' hx with hx hx
+      · cases' hx with i hi
+        apply Exists.intro (_¬ _K i (_C G φ))
+        simp only [Finset.mem_singleton, Finset.union_insert, Finset.mem_union, or_false,
+          Finset.insert_union, Finset.union_assoc, Finset.mem_image, mem_toFinset, and_false,
+          exists_false, or_self, Finset.mem_insert, imp.injEq, and_true, K.injEq, exists_eq_right,
+          hi.left, or_true, ← hi.right, true_and]
         exact @iff_iden (formCLC agents) _ _
-      · cases hx with i hi
-        apply Exists.intro (_K i (_C φ_G φ_φ))
-        simp only [hi.left, ←hi.right, Finset.mem_union, Finset.mem_image, mem_to_finset
-                    eq_self_iff_true, and_true, exists_prop, exists_eq_right, exists_false
-                    or_false, or_true, true_and]
+      · cases' hx with i hi
+        apply Exists.intro (_K i (_C G φ))
+        simp only [Finset.mem_singleton, Finset.union_insert, Finset.mem_union, or_false,
+          Finset.insert_union, Finset.union_assoc, Finset.mem_image, mem_toFinset, and_false,
+          exists_false, or_self, Finset.mem_insert, K.injEq, and_true, exists_eq_right, hi.left,
+          or_true, ← hi.right, true_and]
         exact @iff_dni (formCLC agents) _ _
 
 ----------------------------------------------------------
@@ -283,7 +291,7 @@ inductive subformula {agents : Type} : formCLC agents → formCLC agents → Pro
 | and_right       {φ ψ}   : subformula ψ (φ _∧ ψ)
 | imp_left        {φ ψ}   : subformula φ (φ _→ ψ)
 | imp_right       {φ ψ}   : subformula ψ (φ _→ ψ)
-| effectivity {G} {φ}     : subformula φ ('[G] φ)
+| effectivity {G} {φ}     : subformula φ (_[G] φ)
 | knows       {i} {φ}     : subformula φ (_K i φ)
 | common_know {G} {φ}     : subformula φ (_C G φ)
 
@@ -295,123 +303,150 @@ lemma subformula.cl_subset_and_left {agents : Type} [hN : Fintype agents]
   intro x h
   induction φ
   repeat
-  { simp only [cl, Finset.insert_union, Finset.union_insert, Finset.union_assoc, Finset.mem_insert
+    simp only [cl, Finset.insert_union, Finset.union_insert, Finset.union_assoc, Finset.mem_insert,
                 Finset.mem_union, Finset.mem_singleton] at *
-    repeat {cases h, simp only [h, eq_self_iff_true, and_self, false_or, true_or, or_true],}
-    {simp only [h, eq_self_iff_true, and_self, true_or, false_or, or_true]
+    repeat
+      cases' h with h h
+      simp only [h, eq_self_iff_true, and_self, false_or, true_or, or_true]
+    simp only [h, eq_self_iff_true, and_self, true_or, false_or, or_true]
 
 lemma subformula.cl_subset_and_right {agents : Type} [hN : Fintype agents]
   {φ ψ : formCLC agents} : cl ψ ⊆ cl (φ _∧ ψ) := by
   intro x h
   induction φ
-  repeat
-  { simp [cl] at *
-    repeat {cases h, simp [h],}
-    {simp [h]
+  all_goals
+    · simp_all [cl]
 
 lemma subformula.cl_subset_imp_left {agents : Type} [hN : Fintype agents]
   {φ ψ : formCLC agents} : cl φ ⊆ cl (φ _→ ψ) := by
   intro x h
   induction φ
-  repeat
-  { simp [cl] at *
-    repeat {cases h, simp [h],}
-    {simp [h]
+  all_goals
+    simp_all [cl]
+    repeat
+      cases' h with h h
+      simp [h]
+    simp [h]
 
 lemma subformula.cl_subset_imp_right {agents : Type} [hN : Fintype agents]
   {φ ψ : formCLC agents} : cl ψ ⊆ cl (φ _→ ψ) := by
   intro x h
   induction φ
-  repeat
-  { simp [cl] at *
-    repeat {cases h, simp [h],}
-    {simp [h]
+  all_goals
+  · simp [cl] at *
+    repeat
+      cases h
+    simp [h]
+
 
 lemma subformula.cl_subset_effectivity {agents : Type} [hN : Fintype agents]
-  {φ : formCLC agents} {G : Set (agents)} : cl φ ⊆ cl ('[G] φ) := by
+  {φ : formCLC agents} {G : Set (agents)} : cl φ ⊆ cl (_[G] φ) := by
   intro x h
   induction φ
   repeat
-  { simp [cl] at *
-    repeat {cases h, simp [h],}
-    {simp [h]
+  · simp [cl] at *
+    repeat
+      cases' h with h h
+      simp [h]
+    simp [h]
+
 
 lemma subformula.cl_subset_knows {agents : Type} [hN : Fintype agents]
   {φ : formCLC agents} {i : agents}  : cl φ ⊆ cl (_K i φ) := by
   intro x h
   induction φ
   repeat
-  { simp [cl] at *
-    repeat {cases h, simp [h],}
-    {simp [h]
+  · simp [cl] at *
+    repeat
+      cases' h with h h
+      simp [h]
+    simp [h]
 
 lemma subformula.cl_subset_common_know {agents : Type} [hN : Fintype agents]
   {φ : formCLC agents} {G : Set (agents)} : cl φ ⊆ cl (_C G φ) := by
   intro x h
   induction φ
   repeat
-  { simp [cl] at *
-    repeat {cases h, simp [h],}
-    {simp [h]
+  · simp [cl] at *
+    repeat
+      cases' h with h h
+      simp [h]
+    simp [h]
 
 lemma subformula.cl_subset {agents : Type} [hN : Fintype agents]
   {φ ψ : formCLC agents} (h : subformula φ ψ) : cl φ ⊆ cl ψ := by
-  induction h with _ _ _ _ _ h ih ih'
-  { exact Finset.subset.rfl
-  { exact Finset.subset.trans ih ih'
-  { exact subformula.cl_subset_and_left
-  { exact subformula.cl_subset_and_right
-  { exact subformula.cl_subset_imp_left
-  { exact subformula.cl_subset_imp_right
-  { exact subformula.cl_subset_effectivity
-  { exact subformula.cl_subset_knows
-  { exact subformula.cl_subset_common_know
+  induction' h with _ _ _ _ _ _ ih ih'
+  · exact Finset.Subset.refl _
+  · exact Finset.Subset.trans ih ih'
+  · exact subformula.cl_subset_and_left
+  · exact subformula.cl_subset_and_right
+  · exact subformula.cl_subset_imp_left
+  · exact subformula.cl_subset_imp_right
+  · exact subformula.cl_subset_effectivity
+  · exact subformula.cl_subset_knows
+  · exact subformula.cl_subset_common_know
 
 lemma subformula.mem_cl {agents : Type} [hN : Fintype agents]
   {φ ψ : formCLC agents} (h : subformula φ ψ) : φ ∈ cl ψ :=
 h.cl_subset (cl_contains_phi φ)
 
+lemma test (h: List.Mem 1 []) : False := by
+  -- simp at h
+  exact List.ne_nil_of_mem h (by rfl)
+
+-- set_option maxHeartbeats 200000000
 lemma subformula.in_cl_sub {agents : Type} [hN : Fintype agents]
   {φ ψ χ : formCLC agents} (hcl : ψ ∈ cl φ) (hsub : subformula χ ψ) : χ ∈ cl φ := by
-  induction hsub with _ _ _ _ hsub1 hsub2 hih1 hih2
-  { exact hcl
-  { exact hih1 (hih2 hcl)
+  induction' hsub with _ _ _ _ hsub1 hsub2 hih1 hih2
+  · exact hcl
+  · exact hih1 (hih2 hcl)
   all_goals
-  { induction φ
+    induction' φ with n φ ψ ih_φ ih_ψ φ ψ ih_φ ih_ψ G φ ih i φ ih G φ ih
+    all_goals
+      try unfold cl at hcl
+      try unfold cl
     repeat
-    { simp only [cl, Finset.mem_insert, Finset.mem_singleton, or_self] at hcl
-      cases hcl
+      simp only [cl, Finset.mem_insert, Finset.mem_singleton, or_self] at hcl
+      cases' hcl with hcl
+  all_goals
+    try simp only [Finset.mem_singleton, Finset.union_insert, Finset.union_assoc, Finset.mem_union,
+      or_false, Finset.mem_insert, and.injEq] at hcl
+    try cases' hcl with hcl hcl
+    try rw [hcl.1] at *
+    try rw [hcl.2] at *
+    try rw [hcl]
   any_goals
-  { simp only [cl, cl_C, Finset.mem_insert, Finset.mem_union, Finset.mem_singleton
-                Finset.mem_image, exists_false, or_false, false_or] at hcl
-      cases hcl
-  repeat { apply or.elim hcl, all_goals { intro hcl
-  any_goals { split_ifs at hcl
-  any_goals { rw hcl.1 at *, rw hcl.2 at *
-  any_goals { rw h at *
-  any_goals { simp only [cl, Finset.union_assoc, Finset.mem_insert, Finset.mem_union
-                          Finset.mem_singleton, false_or, Finset.mem_insert, Finset.mem_singleton
-                          or_self, or_false, eq_self_iff_true, and_self, or_true
-                          true_or] at hcl
-  any_goals { simp only [cl_C, Finset.mem_union, Finset.mem_image, exists_false, or_self
-                          or_false] at hcl
-  repeat { apply or.elim hcl, all_goals { intro hcl
-  any_goals { rw hcl.1 at *, rw hcl.2 at *
-  any_goals { rw h at *
-  any_goals { solve1 { by_contra, exact hcl
-  any_goals { simp only [cl, φ_ih_φ hcl, Finset.mem_union, true_or, or_true]
-  any_goals { simp only [cl, φ_ih_ψ hcl, Finset.mem_union, true_or, or_true]
-  any_goals { simp only [cl, Finset.mem_union, cl_contains_phi, true_or, or_true]
-  any_goals { simp only [φ_ih hcl, true_or]
-  any_goals { simp only [if_true, Finset.mem_insert, Finset.mem_singleton, or_false
-                          eq_self_iff_true, and_self, or_true, true_or]
-  any_goals { simp only [hcl.1, hcl.2, eq_self_iff_true, cl_contains_phi, and_self
-                          or_false, or_true, true_or]
-  any_goals { simp only [h, if_false, Finset.mem_insert, eq_self_iff_true, and_self
-                          Finset.mem_singleton, and_false, or_false, or_true]
-  any_goals { obtain ⟨i, ⟨hi, hcl⟩⟩ := hcl
-              rw ←hcl.1 at *, rw ←hcl.2 at *
-              simp only [cl_C, or_false, Finset.mem_union, Finset.mem_image, mem_to_finset
-                          eq_self_iff_true, and_true, exists_prop, exists_eq_right, exists_false
-                          mem_to_finset.mp hi, or_true]
-  any_goals { simp only [cl_contains_bot, or_self, true_or]
+    simp only [cl_C, Finset.mem_union, Finset.mem_image, exists_false, or_self, or_false, cl,
+      Finset.union_assoc, false_or, Finset.mem_insert, Finset.mem_singleton, or_self, or_false,
+      eq_self_iff_true, and_self, or_true, true_or] at hcl
+  any_goals
+    simp only [Finset.mem_singleton, Finset.union_insert, Finset.union_assoc, Finset.mem_union,
+      or_false, Finset.mem_insert, cl_contains_phi, true_or, or_true]
+  repeat
+    all_goals
+      try cases' hcl with hcl hcl
+      try split_ifs with h1
+      try split_ifs at hcl with h3
+      try simp only [ih_φ hcl]
+      try simp only[ih_ψ hcl]
+      try simp only [ih hcl]
+    any_goals
+      · simp only [true_or, or_true]
+  any_goals
+    rename_i _ _ _ h
+    by_contra
+    exact List.ne_nil_of_mem h (by rfl)
+  any_goals
+    simp only [cl, Finset.mem_union, Finset.mem_singleton, imp.injEq, cl_contains_phi,
+      cl_contains_bot, if_true, Finset.mem_insert, Finset.mem_singleton, or_false,  or_self,
+      eq_self_iff_true, and_self, true_or, or_true] at *
+  all_goals
+    try cases' hcl with hcl hcl
+    try simp_all only [hcl.1, true_or, or_true]
+    try simp_all only [hcl.2, true_or, or_true]
+  · rename_i h
+    simp only [h, true_or, or_true]
+  any_goals
+    simp_all only [cl_contains_phi, cl_contains_bot, implies_true, not_false_eq_true, and_self,
+      mem_toFinset, false_or, cl_C, Finset.mem_union, Finset.mem_image, K.injEq,
+      and_true, exists_eq_right, and_false, exists_false, or_false, or_true, true_or, or_self]
